Launchbury/ArityEtaExpandInst.thy
@@ -1,0 +1,430 @@
+theory ArityEtaExpandInst
+imports ArityCorrectSestoft EtaExpansion TransformTools AbstractTransform
+begin
+
+lift_definition Aeta_expand :: "Arity \<Rightarrow> exp \<Rightarrow> exp" is "eta_expand".
+
+lemma Aeta_expand_eqvt[eqvt]: "\<pi> \<bullet> Aeta_expand a e = Aeta_expand (\<pi> \<bullet> a) (\<pi> \<bullet> e)"
+  apply (cases a)
+  apply simp
+  apply transfer
+  apply simp
+  done
+
+lemma Aeta_expand_0[simp]: "Aeta_expand 0 e = e"
+  by transfer simp
+
+lemma Aeta_expand_inc[simp]: "Aeta_expand (inc\<cdot>n) e = (Lam [fresh_var e]. Aeta_expand n (App e (fresh_var e)))"
+  apply (simp add: inc_def)
+  by transfer simp
+
+lemma subst_Aeta_expand:
+  "(Aeta_expand n e)[x::=y] = Aeta_expand n e[x::=y]"
+  by transfer (rule subst_eta_expand)
+
+lemma Aeta_expand_correct:
+  assumes "ae ` upds S \<subseteq> {up \<cdot> 0}"  
+  assumes "Astack ae S \<sqsubseteq> a"
+  shows "(\<Gamma>, Aeta_expand a e, S) \<Rightarrow>\<^sup>* (\<Gamma>, e, S)"
+proof-
+  from assms(1)
+  have "arg_prefix S = Rep_Arity (Astack ae S)"
+    by (induction S arbitrary: a rule: arg_prefix.induct) (auto simp add: Arity.zero_Arity.rep_eq[symmetric])
+  also
+  from assms(2)
+  have "Rep_Arity a \<le> Rep_Arity (Astack ae S)" by (metis below_Arity.rep_eq)
+  finally
+  show ?thesis by transfer (rule eta_expansion_correct')
+qed
+
+lemma isLam_Aeta_expand: "isLam e \<Longrightarrow> isLam (Aeta_expand a e)"
+  by transfer (rule isLam_eta_expand)
+
+lemma Aeta_expand_fresh[simp]: "a \<sharp> Aeta_expand n e = a \<sharp> e" by transfer simp
+lemma Aeta_expand_fresh_star[simp]: "a \<sharp>* Aeta_expand n e = a \<sharp>* e" by (auto simp add: fresh_star_def)
+
+interpretation supp_bounded_transform Aeta_expand
+  apply default
+  using Aeta_expand_fresh
+  apply (auto simp add: fresh_def)
+  done
+
+locale ArityEtaExpand = CorrectArityAnalysisLet
+begin
+  lemma Aeta_expand_pres_Aexp:
+  "Aexp (Aeta_expand n e)\<cdot>n = Aexp e\<cdot>n"
+    apply (induction n arbitrary:e rule: Arity_ind)
+    apply simp
+    apply (simp add: Aexp_App Aexp_Lam)
+    apply (subgoal_tac "fresh_var e \<notin> edom (Aexp e\<cdot>(inc\<cdot>n))")
+    apply simp
+    by (metis Aexp_lookup_fresh edomIff fresh_var_fresh)
+
+  sublocale AbstractTransformBound
+    "\<lambda> e x a . inc\<cdot>a"
+    "\<lambda> x e a . pred\<cdot>a"
+    "\<lambda> \<Delta> e a . a"
+    "\<lambda> \<Delta> e a . Aheap \<Delta>\<cdot>(Aexp e\<cdot>a)"
+    "Aeta_expand"
+  apply default
+  apply ((rule eq_reflection)?, perm_simp, rule)+
+  done
+
+  abbreviation Atransform where "Atransform \<equiv> transform"
+
+  lemma the_map_option_domA[simp]: "x \<in> domA \<Gamma> \<Longrightarrow> the (map_option f (map_of \<Gamma> x)) = f (the (map_of \<Gamma> x))"
+    by (induction \<Gamma>) auto
+
+ (*
+  lemma trans_pres_Aexp: "Aexp (Atransform a e)\<cdot>a = Aexp e\<cdot>a"
+  apply (nominal_induct e arbitrary: a  rule: exp_strong_induct)
+  apply (case_tac b)
+  apply simp_all[2]
+  apply (auto simp add: Aexp_App)[1]
+  defer
+  apply (auto cong add: Aexp_Lam)[1]
+  apply simp
+  apply (rule Aexp_Let_cong)
+  apply simp
+  defer
+  apply simp
+  thm Aheap_cong[where \<Gamma> = "map_transform Atransform (Aheap \<Gamma>\<cdot>(Aexp exp\<cdot>a)) \<Gamma>" and \<Gamma>' = \<Gamma> for \<Gamma> exp]
+  apply (subgoal_tac "Aheap (map_transform Atransform (Aheap \<Gamma>\<cdot>(Aexp exp\<cdot>a)) \<Gamma>)\<cdot>(Aexp exp\<cdot>a) = Aheap \<Gamma>\<cdot>(Aexp exp\<cdot>a)")
+  apply simp
+  defer
+  apply (rule Aheap_cong)
+    apply simp
+    apply (simp add: map_of_map_transform option.map_comp)
+  apply (rule Aheap_cong)
+    apply simp
+    apply (simp add: map_of_map_transform option.map_comp Aeta_expand_pres_Aexp)
+  done
+  
+  lemma trans_pres_Aheap: "Aheap (map_transform Atransform (Aheap \<Delta>\<cdot>ae) \<Delta>)\<cdot>ae = (Aheap \<Delta>\<cdot>ae)"
+    by (rule Aheap_cong) (simp_all add: map_of_map_transform trans_pres_Aexp)
+  *)
+
+  (* Check simp rules *)
+  lemma "transform a (App e x) = App (transform (inc\<cdot>a) e) x" by simp
+  lemma "transform a (Lam [x]. e) = Lam [x].(transform (pred\<cdot>a) e)" by simp
+  lemma "transform a (GVar b x) = GVar b x" by (cases b) simp_all
+  lemma "transform a (Terms.Let \<Delta> e) = Let (map_transform Aeta_expand (Aheap \<Delta>\<cdot>(Aexp e\<cdot>a)) (map_transform transform (Aheap \<Delta>\<cdot>(Aexp e\<cdot>a)) \<Delta>))
+           (transform a e)" by (simp del: Let_eq_iff)
+
+lemma supp_transform: "supp (transform a e) \<subseteq> supp e"
+  by (induction rule: transform.induct)
+     (auto simp add: exp_assn.supp Let_supp dest!: set_mp[OF supp_map_transform] set_mp[OF supp_map_transform_step] )
+
+lemma subst_Aeta_expand_transform: "(transform a e)[x ::= y] = transform a e[x ::= y]"
+proof (nominal_induct e avoiding: x y arbitrary: a  rule: exp_strong_induct_set)
+  case (Let \<Delta> body x y)
+    hence *: "x \<notin> domA \<Delta>" "y \<notin> domA \<Delta>" by (auto simp add: fresh_star_def fresh_at_base)
+    
+    note Let
+    moreover                         
+    from * have "Aheap \<Delta>[x::h=y] = Aheap \<Delta>" by (rule Aheap_subst)
+    moreover
+    have "(Aexp body[x::=y]\<cdot>a) f|` domA \<Delta> = (Aexp body\<cdot>a) f|` domA \<Delta>"
+      by (rule Aexp_subst_restr[OF *])
+    hence "Aheap \<Delta>\<cdot>(Aexp body[x::=y]\<cdot>a) = Aheap \<Delta>\<cdot>(Aexp body\<cdot>a)"
+      by (rule Aheap_cong)
+    ultimately
+    show ?case
+    apply (auto simp add: fresh_star_Pair simp del: Let_eq_iff)
+    apply (rule arg_cong2[where f = Let, OF _ refl])
+    apply (subst subst_map_transform)
+    apply (rule subst_Aeta_expand)
+    apply (subst subst_map_transform)
+    apply assumption
+    apply (rule map_transform_cong)
+    apply simp
+    apply (rule map_transform_cong)
+    apply simp
+    apply simp
+    done
+qed (case_tac b, auto)
+
+
+  fun conf_transform :: "(AEnv \<times> Arity) \<Rightarrow> conf \<Rightarrow> conf"
+  where "conf_transform (ae, a) (\<Gamma>, e, S) =
+    (map_transform Aeta_expand ae (map_transform transform ae \<Gamma>), 
+     transform a e,
+     S)"
+
+  inductive_set thunks :: "heap \<Rightarrow> var set" for \<Gamma> where
+    "map_of \<Gamma> x = Some e \<Longrightarrow> \<not> isLam e \<Longrightarrow> x \<in> thunks \<Gamma>"
+
+  lemma Aheap_thunks: "x \<in> thunks \<Gamma> \<Longrightarrow> (Aheap \<Gamma>\<cdot>ae) x = up\<cdot>0"
+    by (metis thunks.cases Aheap_heap3)
+
+  inductive consistent :: "(AEnv \<times> Arity) \<Rightarrow> conf \<Rightarrow> bool" where
+    consistentI[intro!]: 
+    "edom ae \<subseteq> domA \<Gamma> \<union> upds S
+    \<Longrightarrow> upds S \<subseteq> edom ae
+    \<Longrightarrow> Astack ae S \<sqsubseteq> a
+(*    \<Longrightarrow> AEstack ae S \<sqsubseteq> ae  *)
+    \<Longrightarrow> Aexp e \<cdot> a \<sqsubseteq> ae
+    \<Longrightarrow> (\<And> x e. map_of \<Gamma> x = Some e \<Longrightarrow> Aexp' e \<cdot> (ae x) \<sqsubseteq> ae)
+    \<Longrightarrow> (\<And> x e. map_of \<Gamma> x = Some e \<Longrightarrow> \<not> isLam e \<Longrightarrow> ae x = up\<cdot>0)
+    \<Longrightarrow> ae ` ap S \<subseteq> {up\<cdot>0}
+    \<Longrightarrow> ae ` upds S \<subseteq> {up\<cdot>0}
+    \<Longrightarrow> consistent (ae, a) (\<Gamma>, e, S)"  
+  inductive_cases consistentE[elim!]: "consistent (ae, a) (\<Gamma>, e, S)"
+
+    find_theorems supp Atransform
+
+  interpretation supp_bounded_transform transform
+    by default (auto simp add: fresh_def supp_transform)
+  
+  lemma isLam_Aeta_expand_transform[simp]:
+    "isLam (Atransform a e) \<longleftrightarrow> isLam e"
+    by (induction e rule:isLam.induct) (case_tac b, auto)
+
+(*
+  sublocale AbstractConforms step consistent.
+*)
+
+lemma foo:
+  fixes c c' R 
+  assumes "c \<Rightarrow>\<^sup>* c'" and "\<not> boring_step c'" and "consistent (ae,a) c"
+  shows "\<exists>ae' a'. consistent (ae',a') c' \<and> conf_transform (ae,a) c \<Rightarrow>\<^sup>* conf_transform (ae',a') c'"
+using assms
+proof(induction c c' arbitrary: ae a rule:step_induction)
+case (app\<^sub>1 \<Gamma> e x S)
+  from app\<^sub>1 have "consistent (ae, inc\<cdot>a) (\<Gamma>, e, Arg x # S)"  by (fastforce simp add: Aexp_App join_below_iff)
+  moreover
+  have "conf_transform (ae, a) (\<Gamma>, App e x, S) \<Rightarrow> conf_transform (ae, inc\<cdot>a) (\<Gamma>, e, Arg x # S)" by simp rule
+  ultimately
+  show ?case by (blast del: consistentI consistentE)
+next
+case (app\<^sub>2 \<Gamma> y e x S)
+  have "Aexp (e[y ::= x])\<cdot>(pred\<cdot>a) \<sqsubseteq> ae" using app\<^sub>2
+    apply (auto simp add:  join_below_iff)
+    apply (rule below_trans[OF monofun_cfun_fun[OF Aexp_subst_App_Lam]])
+    apply (auto simp add: Aexp_App Aexp_Lam join_below_iff)
+    done
+  hence "consistent (ae, pred \<cdot> a) (\<Gamma>, e[y::=x], S)"  using app\<^sub>2
+    apply  (auto intro!:  below_trans[OF monofun_cfun_fun[OF Aexp_subst_App_Lam]] simp add: Aexp_App join_below_iff monofun_cfun_arg)
+    apply (metis image_eqI singletonD subsetCE)+
+    done
+  moreover
+  have "conf_transform (ae, a) (\<Gamma>, Lam [y]. e, Arg x # S) \<Rightarrow> conf_transform (ae, pred \<cdot> a) (\<Gamma>, e[y::=x], S)" by (simp add: subst_Aeta_expand_transform[symmetric]) rule
+  ultimately
+  show ?case by (blast del: consistentI consistentE)
+next
+case (thunk \<Gamma> x e S)
+  hence "consistent (ae, 0) (delete x \<Gamma>, e, Upd x # S)" using thunk by (fastforce simp add: join_below_iff)
+  moreover
+  {
+  from thunk
+  have "ae x = up\<cdot>0" by auto
+  with  `map_of \<Gamma> x = Some e`
+  have "map_of (map_transform Aeta_expand ae (map_transform Atransform ae \<Gamma>)) x = Some (transform 0 e)"
+    by (simp add: map_of_map_transform)
+  with `\<not> isLam e`
+  have "conf_transform (ae, a) (\<Gamma>, Var x, S) \<Rightarrow> conf_transform (ae, 0) (delete x \<Gamma>, e, Upd x # S)"
+    by (auto simp add: map_transform_delete intro!: step.intros)
+  }
+  ultimately
+  show ?case by (blast del: consistentI consistentE)
+next
+case (lamvar \<Gamma> x e S)
+  from lamvar have "ae ` upds S \<subseteq> {up \<cdot> 0}" by fastforce
+  from lamvar have "Astack ae S \<sqsubseteq> a" by auto
+
+  from lamvar have "Aexp (Var x)\<cdot>a \<sqsubseteq> ae" by auto
+  from below_trans[OF Aexp_Var fun_belowD[OF this] ]
+  have "up\<cdot>a \<sqsubseteq> ae x".
+  then obtain u where "ae x = up\<cdot>u" and "a \<sqsubseteq> u" by (cases "ae x") auto
+
+
+  from this(2)
+  have "Aexp e\<cdot>a \<sqsubseteq> Aexp e\<cdot>u" by (rule monofun_cfun_arg)
+  also have "\<dots> \<sqsubseteq> ae" using `ae x = up \<cdot> u` lamvar by fastforce
+  finally have "Aexp e\<cdot>a \<sqsubseteq> ae" by this simp
+  moreover
+  have "Aexp' e\<cdot>(ae x) \<sqsubseteq> ae" using lamvar by auto
+  hence "Aexp e\<cdot>u \<sqsubseteq> ae" using `ae x = up\<cdot>u` by simp
+  ultimately
+  have "consistent (ae, u) ((x, e) # delete x \<Gamma>, e, S)"
+    using lamvar by (auto  simp add: join_below_iff split:if_splits intro: below_trans[OF _ `a \<sqsubseteq> u`])
+  moreover
+  {
+  from `isLam e`
+  have "isLam (Atransform u e)" by simp
+  hence "isLam (Aeta_expand u (Atransform u e))" by (rule isLam_Aeta_expand)
+  moreover
+  from  `map_of \<Gamma> x = Some e`  `ae x = up \<cdot> u`
+  have "map_of (map_transform Aeta_expand ae (map_transform Atransform ae \<Gamma>)) x = Some (Aeta_expand u (Atransform u e))"
+    by (simp add: map_of_map_transform)
+  ultimately
+  have "conf_transform (ae, a) (\<Gamma>, Var x, S) \<Rightarrow>\<^sup>*
+        ((x, Aeta_expand u (Atransform u e)) # (map_transform Aeta_expand ae (map_transform Atransform ae (delete x \<Gamma>))), Aeta_expand u  (Atransform u e), S)"
+     by (auto intro: lambda_var simp add: map_transform_delete)
+  also have "\<dots> = ((map_transform Aeta_expand ae (map_transform Atransform ae ((x,e) # delete x \<Gamma>))), Aeta_expand u  (Atransform u e), S)"
+    using `ae x = up \<cdot> u` by (simp add: map_transform_Cons)
+  also(subst[rotated]) have "\<dots> \<Rightarrow>\<^sup>* conf_transform (ae, u) ((x, e) # delete x \<Gamma>, e, S)"
+    apply simp
+    by (rule Aeta_expand_correct[OF `ae \` upds S \<subseteq> {up \<cdot> 0}` below_trans[OF `Astack ae S \<sqsubseteq> a` `a \<sqsubseteq> u`]])
+  finally(rtranclp_trans)
+  have "conf_transform (ae, a) (\<Gamma>, Var x, S) \<Rightarrow>\<^sup>* conf_transform (ae, u) ((x, e) # delete x \<Gamma>, e, S)".
+  }
+  ultimately show ?case by (blast del: consistentI consistentE)
+next
+case (var\<^sub>2 \<Gamma> x e S)
+  hence "ae x = up\<cdot>0" by auto
+
+  have "Astack ae (Upd x # S) \<sqsubseteq> a" using var\<^sub>2 by auto
+  with `ae x = up \<cdot> 0`
+  have "a = 0" by auto
+
+  have "consistent (ae, 0) ((x, e) # \<Gamma>, e, S)" using var\<^sub>2
+    by (fastforce  simp add: join_below_iff split:if_splits)
+  moreover
+  have "conf_transform (ae, a) (\<Gamma>, e, Upd x # S) \<Rightarrow> conf_transform (ae, 0) ((x, e) # \<Gamma>, e, S)"
+    using `ae x = up\<cdot>0` `a = 0` var\<^sub>2 by (auto intro!: step.intros simp add: map_transform_Cons)
+  ultimately show ?case by (blast del: consistentI consistentE)
+next
+  case (let\<^sub>1 \<Delta> \<Gamma> e S)
+
+  let ?ae = "Aheap \<Delta> \<cdot> (Aexp e\<cdot>a)"
+  let ?new = "(domA (\<Delta> @ \<Gamma>) \<union> upds S - (domA \<Gamma> \<union> upds S))"
+  have new: "?new = domA \<Delta>"
+    using fresh_distinct[OF let\<^sub>1(1)] fresh_distinct_fv[OF let\<^sub>1(2)]
+    by (auto dest: set_mp[OF ups_fv_subset])
+
+  have "domA \<Delta> \<inter> upds S = {}" using fresh_distinct_fv[OF let\<^sub>1(2)] by (auto dest: set_mp[OF ups_fv_subset])
+  hence *: "\<And> x. x \<in> upds S \<Longrightarrow> x \<notin> edom (Aheap \<Delta>\<cdot>(Aexp e\<cdot>a))"
+    using edom_Aheap[where \<Gamma> = \<Delta> and ae = "Aexp e\<cdot>a"] by auto
+  hence stack: "AEstack (Aheap \<Delta>\<cdot>(Aexp e\<cdot>a) \<squnion> ae) S = AEstack ae S"
+               "Astack (Aheap \<Delta>\<cdot>(Aexp e\<cdot>a) \<squnion> ae) S = Astack ae S"
+    by (auto simp add: edomIff cong: AEstack_cong Astack_cong)
+
+
+  have "edom ae \<subseteq> - domA \<Delta>" using let\<^sub>1(3)
+    using fresh_distinct[OF let\<^sub>1(1)] fresh_distinct_fv[OF let\<^sub>1(2)]
+    by (fastforce dest: set_mp[OF ups_fv_subset])
+  hence "(?ae \<squnion> ae) f|` (- domA \<Delta>) = ae"
+    by (auto simp add: env_restr_join  env_restr_useless disjoint_eq_subset_Compl edom_Aheap)
+  moreover
+  {
+  have "edom (?ae \<squnion> ae) \<subseteq> domA (\<Delta> @ \<Gamma>) \<union> upds S"
+    using let\<^sub>1(3) by (auto dest: set_mp[OF edom_Aheap])
+  moreover
+  have "upds S \<subseteq> edom (?ae \<squnion> ae)"
+    using let\<^sub>1(3) by auto
+  (*
+  moreover
+  have "AEstack ae S \<sqsubseteq> ae" using let\<^sub>1(3) by auto
+  hence "AEstack ae S \<sqsubseteq> ?ae \<squnion> ae" by (metis join_above1 below_refl box_below join_comm)
+  *)
+  moreover
+  { fix x e'
+    assume "map_of \<Delta> x = Some e'"
+    hence "x \<notin> edom ae" using `edom ae \<subseteq> - domA \<Delta>` by (metis Compl_iff contra_subsetD domI dom_map_of_conv_domA)
+    hence "Aexp' e'\<cdot>((?ae \<squnion> ae) x) = Aexp' e'\<cdot>(?ae x)" by (auto simp add: edomIff)
+    also
+    have "Aexp' e'\<cdot>(?ae x) \<sqsubseteq> (Aexp' e'\<cdot>(?ae x) f|` domA \<Delta>) \<squnion> (Aexp' e'\<cdot>(?ae x) f|` (- domA \<Delta>))"
+      by (rule eq_imp_below[OF join_env_restr_UNIV[symmetric]]) auto
+    also
+    from `map_of \<Delta> x = Some e'`
+    have "Aexp' e'\<cdot>(?ae x) f|` domA \<Delta> \<sqsubseteq> ?ae" by (rule Aheap_heap)
+    also
+    from `map_of \<Delta> x = Some e'`
+    find_theorems Aheap name:heap
+    have "Aexp' e'\<cdot>(?ae x) f|` (- domA \<Delta>) \<sqsubseteq> Aexp (Terms.Let \<Delta> e)\<cdot>a" by (rule Aheap_heap2)
+    also
+    have "Aexp (Terms.Let \<Delta> e)\<cdot>a \<sqsubseteq> ae" using let\<^sub>1(3) by auto
+    finally
+    have "Aexp' e'\<cdot>((?ae \<squnion> ae) x) \<sqsubseteq> ?ae \<squnion> ae" by this auto
+  }
+  moreover
+  { fix x e'
+    assume "map_of \<Gamma> x = Some e'"
+    hence "x \<in> domA \<Gamma>" by (metis domI dom_map_of_conv_domA)
+    hence "x \<notin> edom ?ae" using fresh_distinct[OF let\<^sub>1(1)]  by (auto dest: set_mp[OF edom_Aheap])
+    with let\<^sub>1 `map_of \<Gamma> x = Some e'`
+    have "Aexp' e'\<cdot>((?ae \<squnion> ae) x) \<sqsubseteq> ae" by (auto simp add: edomIff)
+    hence "Aexp' e'\<cdot>((?ae \<squnion> ae) x) \<sqsubseteq> ?ae \<squnion> ae" by (metis (erased, hide_lams) "HOLCF-Join-Classes.join_above2" below_trans)
+  }
+  moreover
+  { fix x e'
+    assume "\<not> isLam e'"
+    assume "map_of \<Gamma> x = Some e'"
+    hence "x \<in> domA \<Gamma>" by (metis domI dom_map_of_conv_domA)
+    hence "x \<notin> edom ?ae" using fresh_distinct[OF let\<^sub>1(1)]  by (auto dest: set_mp[OF edom_Aheap])
+    with let\<^sub>1 `map_of \<Gamma> x = Some e'` `\<not> isLam e'`
+    have "(?ae \<squnion> ae) x = up \<cdot>0" by (auto simp add: edomIff)
+  }
+  moreover
+  { fix x e'
+    assume "map_of \<Delta> x = Some e'" and "\<not> isLam e'"
+    hence "?ae x = up \<cdot> 0" using Aheap_heap3 by auto
+    hence "(?ae \<squnion> ae) x = up \<cdot> 0" by simp
+  }
+  moreover
+  have "(?ae \<squnion> ae) ` upds S \<subseteq> {up \<cdot> 0}" using let\<^sub>1 * by fastforce
+  moreover
+  have "(?ae \<squnion> ae) ` ap S \<subseteq> {up \<cdot> 0}" using let\<^sub>1 * by fastforce
+  moreover
+  have "Astack (?ae \<squnion> ae) S \<sqsubseteq> a" unfolding stack using let\<^sub>1 by auto
+  moreover
+  {
+  have "Aexp e\<cdot>a \<sqsubseteq> (Aexp e\<cdot>a f|` domA \<Delta>) \<squnion> (Aexp e\<cdot>a f|` (- domA \<Delta>))"
+    by (rule eq_imp_below[OF join_env_restr_UNIV[symmetric]]) auto
+  also have "Aexp e\<cdot>a f|` (- domA \<Delta>) \<sqsubseteq> Aexp (Terms.Let \<Delta> e)\<cdot>a" by (rule Aexp_Let_above)
+  also have "\<dots> \<sqsubseteq> ae" using let\<^sub>1(3) by auto
+  also have "Aexp e\<cdot>a f|` domA \<Delta> \<sqsubseteq> ?ae" by (rule Aheap_above_arg)
+  finally have "Aexp e\<cdot>a \<sqsubseteq> ?ae \<squnion> ae" by this auto
+  }
+  ultimately
+  have "consistent (?ae \<squnion> ae, a) (\<Delta> @ \<Gamma>, e, S) "
+    by (auto  simp add: stack)
+  }
+  moreover
+  {
+    have "\<And> x. x \<in> domA \<Gamma> \<Longrightarrow> x \<notin> edom (Aheap \<Delta>\<cdot>(Aexp e\<cdot>a))"
+      using fresh_distinct[OF let\<^sub>1(1)]
+      by (auto dest!: set_mp[OF edom_Aheap])
+    hence "map_transform Aeta_expand ((Aheap \<Delta>\<cdot>(Aexp e\<cdot>a)) \<squnion> ae) (map_transform Atransform ((Aheap \<Delta>\<cdot>(Aexp e\<cdot>a)) \<squnion> ae) \<Gamma>)
+       = map_transform Aeta_expand ae (map_transform Atransform ae \<Gamma>)"
+      by (auto intro!: map_transform_cong simp add: edomIff)
+    moreover
+    from let\<^sub>1 have *: "edom ae \<subseteq> domA \<Gamma> \<union> upds S" by auto
+    have "\<And> x. x \<in> domA \<Delta> \<Longrightarrow> x \<notin> edom ae"
+       using fresh_distinct[OF let\<^sub>1(1)] fresh_distinct_fv[OF let\<^sub>1(2)] 
+       by (auto dest!: set_mp[OF *] set_mp[OF ups_fv_subset])
+    hence "map_transform Aeta_expand ((Aheap \<Delta>\<cdot>(Aexp e\<cdot>a)) \<squnion> ae) (map_transform Atransform ((Aheap \<Delta>\<cdot>(Aexp e\<cdot>a)) \<squnion> ae) \<Delta>)
+       = map_transform Aeta_expand ((Aheap \<Delta>\<cdot>(Aexp e\<cdot>a))) (map_transform Atransform ((Aheap \<Delta>\<cdot>(Aexp e\<cdot>a))) \<Delta>)"
+      by (auto intro!: map_transform_cong simp add: edomIff)
+    ultimately
+    have "conf_transform (ae, a) (\<Gamma>, Terms.Let \<Delta> e, S) \<Rightarrow> conf_transform (?ae \<squnion> ae, a) (\<Delta> @ \<Gamma>, e, S)"
+      apply (simp add: map_transform_append)
+      apply rule
+      using let\<^sub>1(1,2)
+      by auto
+  }
+  ultimately
+  show ?case  by (blast del: consistentI consistentE)
+next
+  case refl thus ?case by auto
+next
+  case trans
+    from trans(5)
+    show ?case
+      apply (auto dest!: trans(3,4))
+      apply (metis (poly_guards_query) rtranclp_trans)
+      done
+qed
+
+(*
+  sublocale AbstractTransform step consistent conf_transform
+    apply default
+    using foo
+    apply (auto del: consistentI consistentE)
+    done
+*)
+
+end
+end
+
